Cleanup lambda-calculus examples.

theories/Examples/Lambda/CBVUntyped.v
@@ -2,8 +2,8 @@
 Un(i)typed Call-by-value Lambda Calculus
 ========================================
 
-This file follows very closely its sibling `CBVTyped.v`. It is recommended to read that one first:
-the comments on this one will be quite more terse and focus on the differences.
+This file follows very closely its sibling `CBVTyped.v`. It is recommended to read that
+one first: the comments on this one will be quite more terse and focus on the differences.
 
 .. coq:: none
 |*)
@@ -19,31 +19,33 @@ Set Warnings "-parsing".
 Syntax
 ------
 
-As our framework is "well-typed well-scoped", when we mean untyped, we really mean unityped,
-i.e., we will take the single element set as set of types. Although, the typing rules will not
-be as uninteresting as it would seem. Indeed, as we adopt a single-sided sequent-calculus
-style of presentation, we do give types to continuations (formally negated types), and we thus
-have not one type, but two: the type of terms `⊕` and the type of continuations `⊖`.
+As our framework is "well-typed well-scoped", when we mean untyped, we really mean
+unityped, i.e., we will take the single element set as set of types. Although, the
+typing rules will not be as uninteresting as it would seem. Indeed, as we adopt a
+single-sided sequent-calculus style of presentation, we do give types to continuations
+(formally negated types), and we thus have not one type, but two: the type of terms
+`⊕` and the type of continuations `⊖`.
 
-Typing contexts, terms, values, evaluation contexts and configurations work straightforwardly.
+Typing contexts, terms, values, evaluation contexts and configurations work
+straightforwardly.
 |*)
 Variant ty : Type :=
-| Tpro : ty
-| Tkon : ty
+| Left : ty
+| Right : ty
 .
-Notation "⊕" := (Tpro) (at level 20) : ty_scope .
-Notation "⊖" := (Tkon) (at level 20) : ty_scope .
-
+Notation "⊕" := (Left) (at level 20) : ty_scope .
+Notation "⊖" := (Right) (at level 20) : ty_scope .
+(*| .. coq:: none |*)
 Declare Scope ty_scope .
 Derive NoConfusion for ty .
 Bind Scope ty_scope with ty .
 Open Scope ty_scope .
-
+(*||*)
 Definition t_ctx : Type := Ctx.ctx ty .
 Bind Scope ctx_scope with t_ctx .
 (*|
-Note that is is the proper pure untyped lambda calculus: in constrast with our ULC example,
-the lambda is not recursive and there is no unit value, only functions.
+Note that is is the proper pure untyped lambda calculus: in constrast with our STLC example,
+the lambda is not recursive and there is no unit value nor base type, only functions.
 |*)
 Inductive term (Γ : t_ctx) : Type :=
 | Val : val Γ -> term Γ
@@ -52,27 +54,30 @@ with val (Γ : t_ctx) : Type :=
 | Var : Γ ∋ ⊕ -> val Γ
 | Lam : term (Γ ▶ₓ ⊕) -> val Γ
 .
+(*| .. coq:: none |*)
 Arguments Val {Γ} & v .
 Arguments App {Γ} & t1 t2 .
 Arguments Var {Γ} & i .
 Arguments Lam {Γ} & t .
-
+(*||*)
 Inductive ev_ctx (Γ : t_ctx) : Type :=
 | K0 : Γ ∋ ⊖ -> ev_ctx Γ
 | K1 : term Γ -> ev_ctx Γ -> ev_ctx Γ
 | K2 : val Γ -> ev_ctx Γ -> ev_ctx Γ
 .
-Arguments K0 {Γ} i .
-Arguments K1 {Γ} t π .
-Arguments K2 {Γ} v π .
-
+(*| .. coq:: none |*)
+Arguments K0 {Γ} & i .
+Arguments K1 {Γ} & t π .
+Arguments K2 {Γ} & v π .
+(*||*)
 Variant state (Γ : t_ctx) : Type :=
 | Cut : term Γ -> ev_ctx Γ -> state Γ
 .
+(*| .. coq:: none |*)
 Arguments Cut {Γ} t π.
-
 (*|
-The sorted family of generalized values.
+We introduce the sorted family of generalized values, together with the generalized
+variable.
 |*)
 Equations val_m : t_ctx -> ty -> Type :=
   val_m Γ (⊕) := val Γ ;
@@ -108,64 +113,24 @@ Renaming an assigment on the left.
 |*)
 Definition a_ren {Γ1 Γ2 Γ3} : Γ1 =[val_m]> Γ2 -> Γ2 ⊆ Γ3 -> Γ1 =[val_m]> Γ3 :=
   fun f g _ i => m_rename g _ (f _ i) .
+Arguments a_ren _ _ _ /.
 (*|
 The following bunch of notations will help us to keep the code readable:
 |*)
 Notation "t ₜ⊛ᵣ r" := (t_rename r%asgn t) (at level 14).
 Notation "v ᵥ⊛ᵣ r" := (v_rename r%asgn v) (at level 14).
 Notation "π ₑ⊛ᵣ r" := (e_rename r%asgn π) (at level 14).
-Notation "v ₘ⊛ᵣ r" := (m_rename r%asgn v) (at level 14).
+Notation "v ₘ⊛ᵣ r" := (m_rename r%asgn _ v) (at level 14).
 Notation "s ₛ⊛ᵣ r" := (s_rename r%asgn s) (at level 14).
-Notation "a ⊛ᵣ r" := (a_ren r%asgn a) (at level 14) : asgn_scope.
+Notation "a ⊛ᵣ r" := (a_ren a%asgn r%asgn) (at level 14) : asgn_scope.
 (*|
 The weakenings we will need for substitution..
 |*)
 Definition t_shift1 {Γ a} := @t_rename Γ (Γ ▶ₓ a) r_pop.
+Definition v_shift1 {Γ a} := @v_rename Γ (Γ ▶ₓ a) r_pop.
 Definition m_shift1 {Γ a} := @m_rename Γ (Γ ▶ₓ a) r_pop.
 Definition a_shift1 {Γ Δ a} (f : Γ =[val_m]> Δ) :=
   [ a_map f m_shift1 ,ₓ a_id a top ]%asgn .
-
-(*|
-Example terms.
-|*)
-Equations n_ctx : nat -> t_ctx :=
-  n_ctx O     := ∅ ;
-  n_ctx (S n) := n_ctx n ▶ₓ ⊕ .
-
-Notation var' n := (n_ctx n ∋ ⊕).
-Notation term' n := (term (n_ctx n)).
-
-Equations v_emb (n : nat) : var' (S n) :=
-  v_emb O     := top ;
-  v_emb (S n) := pop (v_emb n) .
-
-Equations v_lift {n} : var' n -> var' (S n) :=
-  @v_lift (S _) top     := top ;
-  @v_lift (S _) (pop i) := pop (v_lift i) .
-
-Equations mk_var (m : nat) : forall n, var' (m + S n) :=
-  mk_var O     := v_emb ;
-  mk_var (S m) := v_lift ∘ mk_var m .
-
-Definition mk_lam {m : nat} (f : (forall n, term' (m + S n)) -> term' (S m)) : term' m
-  := Val (Lam (f (Val ∘ Var ∘ mk_var m))).
-Arguments mk_lam {_} & _ .
-
-Declare Custom Entry lambda.
-Notation "✨ e ✨" := (e : term' 0) (e custom lambda at level 2).
-Notation "x" := (x _) (in custom lambda at level 0, x ident).
-Notation "( x )" := x (in custom lambda at level 0, x at level 2).
-Notation "x y" := (App x y)
-  (in custom lambda at level 1, left associativity).
-Notation "'λ' x .. y ⇒ U" :=
-  (mk_lam (fun x => .. (mk_lam (fun y => U)) ..))
-  (in custom lambda at level 1, x binder, y binder, U at level 2).
-
-Definition Delta := ✨ (λ x ⇒ x x) ✨ .
-Definition Omega := ✨ (λ x ⇒ x x) (λ x ⇒ x x) ✨ .
-Definition Upsilon := ✨ λ f ⇒ (λ x ⇒ f (x x)) (λ x ⇒ f (x x)) ✨.
-Definition Theta := ✨ (λ x f ⇒ f (x x f)) (λ x f ⇒ f (x x f)) ✨.
-
 (*|
 Substitutions
 ^^^^^^^^^^^^^
@@ -190,9 +155,8 @@ Equations m_subst : val_m ⇒₁ ⟦ val_m , val_m ⟧₁ :=
   m_subst _ (⊕) v _ f := v `ᵥ⊛ f ;
   m_subst _ (⊖) π _ f := π `ₑ⊛ f .
 
-Definition s_subst : state ⇒₀ ⟦ val_m , state ⟧₀ :=
-  fun _ '(Cut t π) _ f => Cut (t `ₜ⊛ f) (π `ₑ⊛ f) .
-
+Equations s_subst : state ⇒₀ ⟦ val_m , state ⟧₀ :=
+  s_subst _ (Cut t π) _ f := Cut (t `ₜ⊛ f) (π `ₑ⊛ f) .
 (*|
 We can now instanciate the substitution monoid and module structures.
 |*)
@@ -316,152 +280,152 @@ Qed.
 Renaming respects pointwise equality of assignments.
 |*)
 Definition t_ren_proper_P Γ (t : term Γ) : Prop :=
-  forall Δ (f1 f2 : Γ ⊆ Δ), f1 ≡ₐ f2 -> f1 ᵣ⊛ₜ t = f2 ᵣ⊛ₜ t .
+  forall Δ (f1 f2 : Γ ⊆ Δ), f1 ≡ₐ f2 -> t ₜ⊛ᵣ f1 = t ₜ⊛ᵣ f2 .
 Definition v_ren_proper_P Γ (v : val Γ) : Prop :=
-  forall Δ (f1 f2 : Γ ⊆ Δ), f1 ≡ₐ f2 -> f1 ᵣ⊛ᵥ v = f2 ᵣ⊛ᵥ v .
+  forall Δ (f1 f2 : Γ ⊆ Δ), f1 ≡ₐ f2 -> v ᵥ⊛ᵣ f1 = v ᵥ⊛ᵣ f2 .
 Definition e_ren_proper_P Γ (π : ev_ctx Γ) : Prop :=
-  forall Δ (f1 f2 : Γ ⊆ Δ), f1 ≡ₐ f2 -> f1 ᵣ⊛ₑ π = f2 ᵣ⊛ₑ π .
+  forall Δ (f1 f2 : Γ ⊆ Δ), f1 ≡ₐ f2 -> π ₑ⊛ᵣ f1 = π ₑ⊛ᵣ f2 .
 Lemma ren_proper_prf : syn_ind_args t_ren_proper_P v_ren_proper_P e_ren_proper_P.
   econstructor.
   all: unfold t_ren_proper_P, v_ren_proper_P, e_ren_proper_P.
   all: intros; cbn; f_equal; auto.
   all: apply H.
-  now apply r_shift_eq.
+  now apply r_shift1_eq.
 Qed.
 
 #[global] Instance t_ren_eq {Γ Δ}
-  : Proper (ass_eq _ _ ==> eq ==> eq) (@t_rename Γ Δ).
+  : Proper (asgn_eq _ _ ==> eq ==> eq) (@t_rename Γ Δ).
   intros f1 f2 H1 x y ->; now apply (term_ind_mut _ _ _ ren_proper_prf).
 Qed.
 #[global] Instance v_ren_eq {Γ Δ}
-  : Proper (ass_eq _ _ ==> eq ==> eq) (@v_rename Γ Δ).
+  : Proper (asgn_eq _ _ ==> eq ==> eq) (@v_rename Γ Δ).
   intros f1 f2 H1 x y ->; now apply (val_ind_mut _ _ _ ren_proper_prf).
 Qed.
 #[global] Instance e_ren_eq {Γ Δ}
-  : Proper (ass_eq _ _ ==> eq ==> eq) (@e_rename Γ Δ).
+  : Proper (asgn_eq _ _ ==> eq ==> eq) (@e_rename Γ Δ).
   intros f1 f2 H1 x y ->; now apply (ctx_ind_mut _ _ _ ren_proper_prf).
 Qed.
 #[global] Instance m_ren_eq {Γ Δ}
-  : Proper (ass_eq _ _ ==> forall_relation (fun a => eq ==> eq)) (@m_rename Γ Δ).
+  : Proper (asgn_eq _ _ ==> forall_relation (fun a => eq ==> eq)) (@m_rename Γ Δ).
   intros ? ? H1 [] _ ? ->; cbn in *; now rewrite H1.
 Qed.
 #[global] Instance s_ren_eq {Γ Δ}
-  : Proper (ass_eq _ _ ==> eq ==> eq) (@s_rename Γ Δ).
+  : Proper (asgn_eq _ _ ==> eq ==> eq) (@s_rename Γ Δ).
   intros ? ? H1 _ x ->; destruct x; cbn; now rewrite H1.
 Qed.
 #[global] Instance a_ren_eq {Γ1 Γ2 Γ3}
-  : Proper (ass_eq _ _ ==> ass_eq _ _ ==> ass_eq _ _) (@a_ren Γ1 Γ2 Γ3).
-  intros ? ? H1 ? ? H2 ? ?; apply (m_ren_eq _ _ H1), H2.
+  : Proper (asgn_eq _ _ ==> asgn_eq _ _ ==> asgn_eq _ _) (@a_ren Γ1 Γ2 Γ3).
+  intros ?? H1 ?? H2 ??; apply (m_ren_eq _ _ H2), H1.
 Qed.
-#[global] Instance a_shift_eq {Γ Δ x} : Proper (ass_eq _ _ ==> ass_eq _ _) (@a_shift Γ Δ x).
-  intros ? ? H ? h.
-  dependent elimination h; cbn; auto.
-  unfold s_map; now rewrite H.
+#[global] Instance a_shift_eq {Γ Δ x} : Proper (asgn_eq _ _ ==> asgn_eq _ _) (@a_shift1 Γ Δ x).
+  intros ? ? H ? h; dependent elimination h; cbn; auto.
+  now rewrite H.
 Qed.
 (*|
 Renaming-renaming assocativity.
 |*)
 Definition t_ren_ren_P Γ1 (t : term Γ1) : Prop :=
-  forall Γ2 Γ3 (f1 : Γ2 ⊆ Γ3) (f2 : Γ1 ⊆ Γ2),
-    f1 ᵣ⊛ₜ (f2 ᵣ⊛ₜ t) = (f1 ⊛ᵣ f2) ᵣ⊛ₜ t .
+  forall Γ2 Γ3 (f1 : Γ1 ⊆ Γ2) (f2 : Γ2 ⊆ Γ3),
+    (t ₜ⊛ᵣ f1) ₜ⊛ᵣ f2 = t ₜ⊛ᵣ (f1 ᵣ⊛ f2)  .
 Definition v_ren_ren_P Γ1 (v : val Γ1) : Prop :=
-  forall Γ2 Γ3 (f1 : Γ2 ⊆ Γ3) (f2 : Γ1 ⊆ Γ2),
-    f1 ᵣ⊛ᵥ (f2 ᵣ⊛ᵥ v) = (f1 ⊛ᵣ f2) ᵣ⊛ᵥ v .
+  forall Γ2 Γ3 (f1 : Γ1 ⊆ Γ2) (f2 : Γ2 ⊆ Γ3),
+    (v ᵥ⊛ᵣ f1) ᵥ⊛ᵣ f2 = v ᵥ⊛ᵣ (f1 ᵣ⊛ f2)  .
 Definition e_ren_ren_P Γ1 (π : ev_ctx Γ1) : Prop :=
-  forall Γ2 Γ3 (f1 : Γ2 ⊆ Γ3) (f2 : Γ1 ⊆ Γ2),
-    f1 ᵣ⊛ₑ (f2 ᵣ⊛ₑ π) = (f1 ⊛ᵣ f2) ᵣ⊛ₑ π .
+  forall Γ2 Γ3 (f1 : Γ1 ⊆ Γ2) (f2 : Γ2 ⊆ Γ3),
+    (π ₑ⊛ᵣ f1) ₑ⊛ᵣ f2 = π ₑ⊛ᵣ (f1 ᵣ⊛ f2)  .
 
 Lemma ren_ren_prf : syn_ind_args t_ren_ren_P v_ren_ren_P e_ren_ren_P .
   econstructor.
   all: unfold t_ren_ren_P, v_ren_ren_P, e_ren_ren_P.
   all: intros; cbn; f_equal; auto.
-  all: now repeat rewrite r_shift_comp.
+  rewrite H; apply t_ren_eq; auto.
+  intros ? h; dependent elimination h; auto.
 Qed.
 
-Lemma t_ren_ren {Γ1 Γ2 Γ3} (f1 : Γ2 ⊆ Γ3) (f2 : Γ1 ⊆ Γ2) (t : term Γ1)
-  : f1 ᵣ⊛ₜ (f2 ᵣ⊛ₜ t) = (f1 ⊛ᵣ f2) ᵣ⊛ₜ t .
+Lemma t_ren_ren {Γ1 Γ2 Γ3} (f1 : Γ1 ⊆ Γ2) (f2 : Γ2 ⊆ Γ3) (t : term Γ1)
+  : (t ₜ⊛ᵣ f1) ₜ⊛ᵣ f2 = t ₜ⊛ᵣ (f1 ᵣ⊛ f2)  .
   now apply (term_ind_mut _ _ _ ren_ren_prf).
 Qed.
-Lemma v_ren_ren {Γ1 Γ2 Γ3} (f1 : Γ2 ⊆ Γ3) (f2 : Γ1 ⊆ Γ2) (v : val Γ1)
-  : f1 ᵣ⊛ᵥ (f2 ᵣ⊛ᵥ v) = (f1 ⊛ᵣ f2) ᵣ⊛ᵥ v .
+Lemma v_ren_ren {Γ1 Γ2 Γ3} (f1 : Γ1 ⊆ Γ2) (f2 : Γ2 ⊆ Γ3) (v : val Γ1)
+  : (v ᵥ⊛ᵣ f1) ᵥ⊛ᵣ f2 = v ᵥ⊛ᵣ (f1 ᵣ⊛ f2)  .
   now apply (val_ind_mut _ _ _ ren_ren_prf).
 Qed.
-Lemma e_ren_ren {Γ1 Γ2 Γ3} (f1 : Γ2 ⊆ Γ3) (f2 : Γ1 ⊆ Γ2) (π : ev_ctx Γ1)
-  : f1 ᵣ⊛ₑ (f2 ᵣ⊛ₑ π) = (f1 ⊛ᵣ f2) ᵣ⊛ₑ π .
+Lemma e_ren_ren {Γ1 Γ2 Γ3} (f1 : Γ1 ⊆ Γ2) (f2 : Γ2 ⊆ Γ3) (π : ev_ctx Γ1)
+  : (π ₑ⊛ᵣ f1) ₑ⊛ᵣ f2 = π ₑ⊛ᵣ (f1 ᵣ⊛ f2)  .
   now apply (ctx_ind_mut _ _ _ ren_ren_prf).
 Qed.
-Lemma m_ren_ren {Γ1 Γ2 Γ3} (f1 : Γ2 ⊆ Γ3) (f2 : Γ1 ⊆ Γ2) a (v : val_m Γ1 a)
-  : f1 ᵣ⊛ₘ (f2 ᵣ⊛ₘ v) = (f1 ⊛ᵣ f2) ᵣ⊛ₘ v .
+Lemma m_ren_ren {Γ1 Γ2 Γ3} (f1 : Γ1 ⊆ Γ2) (f2 : Γ2 ⊆ Γ3) a (v : val_m Γ1 a)
+  : (v ₘ⊛ᵣ f1) ₘ⊛ᵣ f2 = v ₘ⊛ᵣ (f1 ᵣ⊛ f2)  .
   destruct a; [ now apply v_ren_ren | now apply e_ren_ren ].
 Qed.
-Lemma s_ren_ren {Γ1 Γ2 Γ3} (f1 : Γ2 ⊆ Γ3) (f2 : Γ1 ⊆ Γ2) (s : state Γ1)
-  : f1 ᵣ⊛ₛ (f2 ᵣ⊛ₛ s) = (f1 ⊛ᵣ f2) ᵣ⊛ₛ s .
+Lemma s_ren_ren {Γ1 Γ2 Γ3} (f1 : Γ1 ⊆ Γ2) (f2 : Γ2 ⊆ Γ3) (s : state Γ1)
+  : (s ₛ⊛ᵣ f1) ₛ⊛ᵣ f2 = s ₛ⊛ᵣ (f1 ᵣ⊛ f2)  .
   destruct s; apply (f_equal2 Cut); [ now apply t_ren_ren | now apply e_ren_ren ].
 Qed.
 (*|
 Left identity law of renaming.
 |*)
-Definition t_ren_id_l_P Γ (t : term Γ) : Prop := r_id ᵣ⊛ₜ t = t .
-Definition v_ren_id_l_P Γ (v : val Γ) : Prop := r_id ᵣ⊛ᵥ v = v .
-Definition e_ren_id_l_P Γ (π : ev_ctx Γ) : Prop := r_id ᵣ⊛ₑ π = π .
+Definition t_ren_id_l_P Γ (t : term Γ) : Prop := t ₜ⊛ᵣ r_id = t .
+Definition v_ren_id_l_P Γ (v : val Γ) : Prop := v ᵥ⊛ᵣ r_id = v .
+Definition e_ren_id_l_P Γ (π : ev_ctx Γ) : Prop := π ₑ⊛ᵣ r_id = π .
 Lemma ren_id_l_prf : syn_ind_args t_ren_id_l_P v_ren_id_l_P e_ren_id_l_P .
   econstructor.
   all: unfold t_ren_id_l_P, v_ren_id_l_P, e_ren_id_l_P.
   all: intros; cbn; f_equal; auto.
-  now repeat rewrite r_shift_id.
+  rewrite <- H at 2; apply t_ren_eq; auto.
+  intros ? h; dependent elimination h; auto.
 Qed.
 
-Lemma t_ren_id_l {Γ} (t : term Γ) : r_id ᵣ⊛ₜ t = t .
+Lemma t_ren_id_l {Γ} (t : term Γ) : t ₜ⊛ᵣ r_id = t.
   now apply (term_ind_mut _ _ _ ren_id_l_prf).
 Qed.
-Lemma v_ren_id_l {Γ} (v : val Γ) : r_id ᵣ⊛ᵥ v = v .
+Lemma v_ren_id_l {Γ} (v : val Γ) : v ᵥ⊛ᵣ r_id = v .
   now apply (val_ind_mut _ _ _ ren_id_l_prf).
 Qed.
-Lemma e_ren_id_l {Γ} (π : ev_ctx Γ) : r_id ᵣ⊛ₑ π = π .
+Lemma e_ren_id_l {Γ} (π : ev_ctx Γ) : π ₑ⊛ᵣ r_id = π.
   now apply (ctx_ind_mut _ _ _ ren_id_l_prf).
 Qed.
-Lemma m_ren_id_l {Γ a} (v : val_m Γ a) : r_id ᵣ⊛ₘ v = v .
+Lemma m_ren_id_l {Γ a} (v : val_m Γ a) : v ₘ⊛ᵣ r_id = v .
   destruct a; [ now apply v_ren_id_l | now apply e_ren_id_l ].
 Qed.
-Lemma s_ren_id_l {Γ} (s : state Γ) : r_id ᵣ⊛ₛ s = s .
+Lemma s_ren_id_l {Γ} (s : state Γ) : s ₛ⊛ᵣ r_id = s .
   destruct s; apply (f_equal2 Cut); [ now apply t_ren_id_l | now apply e_ren_id_l ].
 Qed.
-(*|
-Right identity law of renaming.
-|*)
-Lemma m_ren_id_r {Γ Δ} (f : Γ ⊆ Δ) {a} (i : Γ ∋ a) : f ᵣ⊛ₘ a_id a i = a_id a (f a i) .
+
+Lemma m_ren_id_r {Γ Δ} (f : Γ ⊆ Δ) {a} (i : Γ ∋ a) : a_id _ i ₘ⊛ᵣ f = a_id _ (f _ i) .
   now destruct a.
 Qed.
-Lemma a_ren_id_r {Γ Δ} (f : Γ ⊆ Δ) : f ᵣ⊛ a_id ≡ₐ a_id ⊛ᵣ f .
-  intros ? ?; now apply m_ren_id_r.
+
+Lemma a_ren_id_r {Γ Δ} (f : Γ ⊆ Δ) : a_id ⊛ᵣ f ≡ₐ f ᵣ⊛ a_id .
+  intros ??; now apply m_ren_id_r.
 Qed.
-Lemma a_shift_id {Γ x} : @a_shift Γ Γ x a_id ≡ₐ a_id.
-  unfold a_shift, m_shift; intros ? h.
-  dependent elimination h; cbn; auto.
+Lemma a_shift_id {Γ x} : @a_shift1 Γ Γ x a_id ≡ₐ a_id.
+  intros ? v; dependent elimination v; auto.
   exact (m_ren_id_r _ _).
 Qed.
 (*|
-Shifting assigments commutes with left and right renaming.
+Lemma 5: shifting assigments commutes with left and right renaming.
 |*)
-Lemma a_shift_s_ren {Γ1 Γ2 Γ3 a} (f1 : Γ2 =[val_m]> Γ3) (f2 : Γ1 ⊆ Γ2)
-  : @a_shift _ _ a (f1 ⊛ᵣ f2) ≡ₐ a_shift f1 ⊛ᵣ r_shift f2 .
-  intros ? h; dependent elimination h; auto.
+Lemma a_shift1_s_ren {Γ1 Γ2 Γ3 a} (f1 : Γ1 ⊆ Γ2) (f2 : Γ2 =[val_m]> Γ3)
+  : @a_shift1 _ _ a (f1 ᵣ⊛ f2) ≡ₐ r_shift1 f1 ᵣ⊛ a_shift1 f2 .
+  intros ? v; dependent elimination v; auto.
 Qed.
-Lemma a_shift_a_ren {Γ1 Γ2 Γ3 a} (f1 : Γ2 ⊆ Γ3) (f2 : Γ1 =[val_m]> Γ2)
-      : @a_shift _ _ a (f1 ᵣ⊛ f2) ≡ₐ r_shift f1 ᵣ⊛ a_shift f2 .
-  unfold r_shift, r_shift, a_shift, m_shift, a_ren; intros ? h.
-  dependent elimination h; cbn; [ symmetry; exact (a_ren_id_r _ _ _) | ].
-  unfold s_map; now rewrite 2 m_ren_ren.
+Lemma a_shift1_a_ren {Γ1 Γ2 Γ3 a} (f1 : Γ1 =[val_m]> Γ2) (f2 : Γ2 ⊆ Γ3)
+      : @a_shift1 _ _ a (f1 ⊛ᵣ f2) ≡ₐ a_shift1 f1 ⊛ᵣ r_shift1 f2 .
+  intros ? v.
+  dependent elimination v.
+  cbn; now rewrite m_ren_id_r.
+  cbn; unfold m_shift1, r_shift1; now rewrite 2 m_ren_ren.
 Qed.
 (*|
-Substitution respects pointwise equality of assigments.
+Lemma 6: substitution respects pointwise equality of assigments.
 |*)
 Definition t_sub_proper_P Γ (t : term Γ) : Prop :=
-  forall Δ (f1 f2 : Γ =[val_m]> Δ), f1 ≡ₐ f2 -> f1 ⊛ₜ t = f2 ⊛ₜ t .
+  forall Δ (f1 f2 : Γ =[val_m]> Δ), f1 ≡ₐ f2 -> t `ₜ⊛ f1 = t `ₜ⊛ f2 .
 Definition v_sub_proper_P Γ (v : val Γ) : Prop :=
-  forall Δ (f1 f2 : Γ =[val_m]> Δ), f1 ≡ₐ f2 -> f1 ⊛ᵥ v = f2 ⊛ᵥ v .
+  forall Δ (f1 f2 : Γ =[val_m]> Δ), f1 ≡ₐ f2 -> v `ᵥ⊛ f1 = v `ᵥ⊛ f2 .
 Definition e_sub_proper_P Γ (π : ev_ctx Γ) : Prop :=
-  forall Δ (f1 f2 : Γ =[val_m]> Δ), f1 ≡ₐ f2 -> f1 ⊛ₑ π = f2 ⊛ₑ π .
+  forall Δ (f1 f2 : Γ =[val_m]> Δ), f1 ≡ₐ f2 -> π `ₑ⊛ f1 = π `ₑ⊛ f2.
 Lemma sub_proper_prf : syn_ind_args t_sub_proper_P v_sub_proper_P e_sub_proper_P.
   econstructor.
   all: unfold t_sub_proper_P, v_sub_proper_P, e_sub_proper_P.
@@ -470,363 +434,289 @@ Lemma sub_proper_prf : syn_ind_args t_sub_proper_P v_sub_proper_P e_sub_proper_P
 Qed.
 
 #[global] Instance t_sub_eq {Γ Δ}
-  : Proper (ass_eq _ _ ==> eq ==> eq) (@t_subst Γ Δ).
+  : Proper (asgn_eq _ _ ==> eq ==> eq) (@t_subst Γ Δ).
   intros ? ? H1 _ ? ->; now apply (term_ind_mut _ _ _ sub_proper_prf).
 Qed.
 #[global] Instance v_sub_eq {Γ Δ}
-  : Proper (ass_eq _ _ ==> eq ==> eq) (@v_subst Γ Δ).
+  : Proper (asgn_eq _ _ ==> eq ==> eq) (@v_subst Γ Δ).
   intros ? ? H1 _ ? ->; now apply (val_ind_mut _ _ _ sub_proper_prf).
 Qed.
 #[global] Instance e_sub_eq {Γ Δ}
-  : Proper (ass_eq _ _ ==> eq ==> eq) (@e_subst Γ Δ).
+  : Proper (asgn_eq _ _ ==> eq ==> eq) (@e_subst Γ Δ).
   intros ? ? H1 _ ? ->; now apply (ctx_ind_mut _ _ _ sub_proper_prf).
 Qed.
-#[global] Instance m_sub_eq {Γ Δ}
-  : Proper (ass_eq _ _ ==> forall_relation (fun a => eq ==> eq)) (@m_subst Γ Δ).
-  intros ? ? H1 [] _ ? ->; cbn in *; now rewrite H1.
+#[global] Instance m_sub_eq
+  : Proper (∀ₕ Γ, ∀ₕ _, eq ==> ∀ₕ Δ, asgn_eq Γ Δ ==> eq) m_subst.
+  intros ? [] ?? -> ??? H1; cbn in *; now rewrite H1.
 Qed.
-#[global] Instance s_sub_eq {Γ Δ}
-  : Proper (ass_eq _ _ ==> eq ==> eq) (@s_subst Γ Δ).
-  intros ? ? H1 _ x ->; destruct x; cbn; now rewrite H1.
+#[global] Instance s_sub_eq
+  : Proper (∀ₕ Γ, eq ==> ∀ₕ Δ, asgn_eq Γ Δ ==> eq) s_subst.
+  intros ??[] -> ??? H1; cbn; now rewrite H1.
 Qed.
+(*
 #[global] Instance a_comp_eq {Γ1 Γ2 Γ3} : Proper (ass_eq _ _ ==> ass_eq _ _ ==> ass_eq _ _) (@a_comp Γ1 Γ2 Γ3).
   intros ? ? H1 ? ? H2 ? ?; unfold a_comp, s_map; now rewrite H1, H2.
 Qed.
+*)
 (*|
-Renaming-substitution "associativity".
+Lemma 7: renaming-substitution "associativity".
 |*)
 Definition t_ren_sub_P Γ1 (t : term Γ1) : Prop :=
-  forall Γ2 Γ3 (f1 : Γ2 ⊆ Γ3) (f2 : Γ1 =[val_m]> Γ2),
-    f1 ᵣ⊛ₜ (f2 ⊛ₜ t) = (f1 ᵣ⊛ f2) ⊛ₜ t .
+  forall Γ2 Γ3 (f1 : Γ1 =[val_m]> Γ2) (f2 : Γ2 ⊆ Γ3) ,
+    (t `ₜ⊛ f1) ₜ⊛ᵣ f2 = t `ₜ⊛ (f1 ⊛ᵣ f2) .
 Definition v_ren_sub_P Γ1 (v : val Γ1) : Prop :=
-  forall Γ2 Γ3 (f1 : Γ2 ⊆ Γ3) (f2 : Γ1 =[val_m]> Γ2),
-    f1 ᵣ⊛ᵥ (f2 ⊛ᵥ v) = (f1 ᵣ⊛ f2) ⊛ᵥ v .
+  forall Γ2 Γ3 (f1 : Γ1 =[val_m]> Γ2) (f2 : Γ2 ⊆ Γ3) ,
+    (v `ᵥ⊛ f1) ᵥ⊛ᵣ f2 = v `ᵥ⊛ (f1 ⊛ᵣ f2) .
 Definition e_ren_sub_P Γ1 (π : ev_ctx Γ1) : Prop :=
-  forall Γ2 Γ3 (f1 : Γ2 ⊆ Γ3) (f2 : Γ1 =[val_m]> Γ2),
-    f1 ᵣ⊛ₑ (f2 ⊛ₑ π) = (f1 ᵣ⊛ f2) ⊛ₑ π .
+  forall Γ2 Γ3 (f1 : Γ1 =[val_m]> Γ2) (f2 : Γ2 ⊆ Γ3) ,
+    (π `ₑ⊛ f1) ₑ⊛ᵣ f2 = π `ₑ⊛ (f1 ⊛ᵣ f2) .
 Lemma ren_sub_prf : syn_ind_args t_ren_sub_P v_ren_sub_P e_ren_sub_P.
   econstructor.
   all: unfold t_ren_sub_P, v_ren_sub_P, e_ren_sub_P.
-  all: intros; cbn; f_equal.
-  all: try rewrite a_shift_a_ren; auto.
+  all: intros; cbn; f_equal; auto.
+  change (a_shift1 (fun x => _)) with (a_shift1 (a:=⊕) (f1 ⊛ᵣ f2)); now rewrite a_shift1_a_ren.
 Qed.
 
-Lemma t_ren_sub {Γ1 Γ2 Γ3} (f1 : Γ2 ⊆ Γ3) (f2 : Γ1 =[val_m]> Γ2) (t : term Γ1)
-  : f1 ᵣ⊛ₜ (f2 ⊛ₜ t) = (f1 ᵣ⊛ f2) ⊛ₜ t .
+Lemma t_ren_sub {Γ1 Γ2 Γ3} (f1 : Γ1 =[val_m]> Γ2) (f2 : Γ2 ⊆ Γ3) (t : term Γ1)
+  : (t `ₜ⊛ f1) ₜ⊛ᵣ f2 = t `ₜ⊛ (f1 ⊛ᵣ f2) .
   now apply (term_ind_mut _ _ _ ren_sub_prf).
 Qed.
-Lemma v_ren_sub {Γ1 Γ2 Γ3} (f1 : Γ2 ⊆ Γ3) (f2 : Γ1 =[val_m]> Γ2) (v : val Γ1)
-  : f1 ᵣ⊛ᵥ (f2 ⊛ᵥ v) = (f1 ᵣ⊛ f2) ⊛ᵥ v .
+Lemma v_ren_sub {Γ1 Γ2 Γ3} (f1 : Γ1 =[val_m]> Γ2) (f2 : Γ2 ⊆ Γ3) (v : val Γ1)
+  : (v `ᵥ⊛ f1) ᵥ⊛ᵣ f2 = v `ᵥ⊛ (f1 ⊛ᵣ f2) .
   now apply (val_ind_mut _ _ _ ren_sub_prf).
 Qed.
-Lemma e_ren_sub {Γ1 Γ2 Γ3} (f1 : Γ2 ⊆ Γ3) (f2 : Γ1 =[val_m]> Γ2) (π : ev_ctx Γ1)
-  : f1 ᵣ⊛ₑ (f2 ⊛ₑ π) = (f1 ᵣ⊛ f2) ⊛ₑ π .
+Lemma e_ren_sub {Γ1 Γ2 Γ3} (f1 : Γ1 =[val_m]> Γ2) (f2 : Γ2 ⊆ Γ3) (π : ev_ctx Γ1)
+  : (π `ₑ⊛ f1) ₑ⊛ᵣ f2 = π `ₑ⊛ (f1 ⊛ᵣ f2) .
   now apply (ctx_ind_mut _ _ _ ren_sub_prf).
 Qed.
-Lemma m_ren_sub {Γ1 Γ2 Γ3} (f1 : Γ2 ⊆ Γ3) (f2 : Γ1 =[val_m]> Γ2) a (v : val_m Γ1 a)
-  : f1 ᵣ⊛ₘ (f2 ⊛ₘ v) = (f1 ᵣ⊛ f2) ⊛ₘ v .
+Lemma m_ren_sub {Γ1 Γ2 Γ3} (f1 : Γ1 =[val_m]> Γ2) (f2 : Γ2 ⊆ Γ3) a (v : val_m Γ1 a)
+  : (v ᵥ⊛ f1) ₘ⊛ᵣ f2 = v ᵥ⊛ (f1 ⊛ᵣ f2) .
   destruct a; [ now apply v_ren_sub | now apply e_ren_sub ].
 Qed.
-Lemma s_ren_sub {Γ1 Γ2 Γ3} (f1 : Γ2 ⊆ Γ3) (f2 : Γ1 =[val_m]> Γ2) (s : state Γ1)
-  : f1 ᵣ⊛ₛ (f2 ⊛ₛ s) = (f1 ᵣ⊛ f2) ⊛ₛ s .
+Lemma s_ren_sub {Γ1 Γ2 Γ3} (f1 : Γ1 =[val_m]> Γ2) (f2 : Γ2 ⊆ Γ3) (s : state Γ1)
+  : (s ₜ⊛ f1) ₛ⊛ᵣ f2 = s ₜ⊛ (f1 ⊛ᵣ f2) .
   destruct s; cbn; now rewrite t_ren_sub, e_ren_sub.
 Qed.
 (*|
-Substitution-renaming "associativity".
+Lemma 8: substitution-renaming "associativity".
 |*)
 Definition t_sub_ren_P Γ1 (t : term Γ1) : Prop :=
-  forall Γ2 Γ3 (f1 : Γ2 =[val_m]> Γ3) (f2 : Γ1 ⊆ Γ2),
-  f1 ⊛ₜ (f2 ᵣ⊛ₜ t) = (f1 ⊛ᵣ f2) ⊛ₜ t .
+  forall Γ2 Γ3 (f1 : Γ1 ⊆ Γ2) (f2 : Γ2 =[val_m]> Γ3) ,
+  (t ₜ⊛ᵣ f1) `ₜ⊛ f2 = t `ₜ⊛ (f1 ᵣ⊛ f2) .
 Definition v_sub_ren_P Γ1 (v : val Γ1) : Prop :=
-  forall Γ2 Γ3 (f1 : Γ2 =[val_m]> Γ3) (f2 : Γ1 ⊆ Γ2),
-  f1 ⊛ᵥ (f2 ᵣ⊛ᵥ v) = (f1 ⊛ᵣ f2) ⊛ᵥ v .
+  forall Γ2 Γ3 (f1 : Γ1 ⊆ Γ2) (f2 : Γ2 =[val_m]> Γ3) ,
+  (v ᵥ⊛ᵣ f1) `ᵥ⊛ f2 = v `ᵥ⊛ (f1 ᵣ⊛ f2) .
 Definition e_sub_ren_P Γ1 (π : ev_ctx Γ1) : Prop :=
-  forall Γ2 Γ3 (f1 : Γ2 =[val_m]> Γ3) (f2 : Γ1 ⊆ Γ2),
-  f1 ⊛ₑ (f2 ᵣ⊛ₑ π) = (f1 ⊛ᵣ f2) ⊛ₑ π .
+  forall Γ2 Γ3 (f1 : Γ1 ⊆ Γ2) (f2 : Γ2 =[val_m]> Γ3) ,
+  (π ₑ⊛ᵣ f1) `ₑ⊛ f2 = π `ₑ⊛ (f1 ᵣ⊛ f2) .
 Lemma sub_ren_prf : syn_ind_args t_sub_ren_P v_sub_ren_P e_sub_ren_P.
   econstructor.
   all: unfold t_sub_ren_P, v_sub_ren_P, e_sub_ren_P.
-  all: intros; cbn; f_equal.
-  all: try rewrite a_shift_s_ren; auto.
+  all: intros; cbn; f_equal; auto.
+  now rewrite a_shift1_s_ren.
 Qed.
 
-Lemma t_sub_ren {Γ1 Γ2 Γ3} (f1 : Γ2 =[val_m]> Γ3) (f2 : Γ1 ⊆ Γ2) (t : term Γ1)
-  : f1 ⊛ₜ (f2 ᵣ⊛ₜ t) = (f1 ⊛ᵣ f2) ⊛ₜ t .
+Lemma t_sub_ren {Γ1 Γ2 Γ3} (f1 : Γ1 ⊆ Γ2) (f2 : Γ2 =[val_m]> Γ3) (t : term Γ1)
+  : (t ₜ⊛ᵣ f1) `ₜ⊛ f2 = t `ₜ⊛ (f1 ᵣ⊛ f2) .
   now apply (term_ind_mut _ _ _ sub_ren_prf).
 Qed.
-Lemma v_sub_ren {Γ1 Γ2 Γ3} (f1 : Γ2 =[val_m]> Γ3) (f2 : Γ1 ⊆ Γ2) (v : val Γ1)
-  : f1 ⊛ᵥ (f2 ᵣ⊛ᵥ v) = (f1 ⊛ᵣ f2) ⊛ᵥ v .
+Lemma v_sub_ren {Γ1 Γ2 Γ3} (f1 : Γ1 ⊆ Γ2) (f2 : Γ2 =[val_m]> Γ3) (v : val Γ1)
+  : (v ᵥ⊛ᵣ f1) `ᵥ⊛ f2 = v `ᵥ⊛ (f1 ᵣ⊛ f2) .
   now apply (val_ind_mut _ _ _ sub_ren_prf).
 Qed.
-Lemma e_sub_ren {Γ1 Γ2 Γ3} (f1 : Γ2 =[val_m]> Γ3) (f2 : Γ1 ⊆ Γ2) (π : ev_ctx Γ1)
-  : f1 ⊛ₑ (f2 ᵣ⊛ₑ π) = (f1 ⊛ᵣ f2) ⊛ₑ π .
+Lemma e_sub_ren {Γ1 Γ2 Γ3} (f1 : Γ1 ⊆ Γ2) (f2 : Γ2 =[val_m]> Γ3) (π : ev_ctx Γ1)
+  : (π ₑ⊛ᵣ f1) `ₑ⊛ f2 = π `ₑ⊛ (f1 ᵣ⊛ f2) .
   now apply (ctx_ind_mut _ _ _ sub_ren_prf).
 Qed.
-Lemma m_sub_ren {Γ1 Γ2 Γ3} (f1 : Γ2 =[val_m]> Γ3) (f2 : Γ1 ⊆ Γ2) a (v : val_m Γ1 a)
-  : f1 ⊛ₘ (f2 ᵣ⊛ₘ v) = (f1 ⊛ᵣ f2) ⊛ₘ v .
+Lemma m_sub_ren {Γ1 Γ2 Γ3} (f1 : Γ1 ⊆ Γ2) (f2 : Γ2 =[val_m]> Γ3) a (v : val_m Γ1 a)
+  : (v ₘ⊛ᵣ f1) ᵥ⊛ f2 = v ᵥ⊛ (f1 ᵣ⊛ f2) .
   destruct a; [ now apply v_sub_ren | now apply e_sub_ren ].
 Qed.
-Lemma s_sub_ren {Γ1 Γ2 Γ3} (f1 : Γ2 =[val_m]> Γ3) (f2 : Γ1 ⊆ Γ2) (s : state Γ1)
-  : f1 ⊛ₛ (f2 ᵣ⊛ₛ s) = (f1 ⊛ᵣ f2) ⊛ₛ s .
+Lemma s_sub_ren {Γ1 Γ2 Γ3} (f1 : Γ1 ⊆ Γ2) (f2 : Γ2 =[val_m]> Γ3) (s : state Γ1)
+  : (s ₛ⊛ᵣ f1) ₜ⊛ f2 = s ₜ⊛ (f1 ᵣ⊛ f2) .
   destruct s; cbn; now rewrite t_sub_ren, e_sub_ren.
 Qed.
 (*|
-Left identity law of substitution.
+Lemma 9: left identity law of substitution.
 |*)
-Definition t_sub_id_l_P Γ (t : term Γ) : Prop := a_id ⊛ₜ t = t .
-Definition v_sub_id_l_P Γ (v : val Γ) : Prop := a_id ⊛ᵥ v = v .
-Definition e_sub_id_l_P Γ (π : ev_ctx Γ) : Prop := a_id ⊛ₑ π = π .
+Definition t_sub_id_l_P Γ (t : term Γ) : Prop := t `ₜ⊛ a_id = t .
+Definition v_sub_id_l_P Γ (v : val Γ) : Prop := v `ᵥ⊛ a_id = v .
+Definition e_sub_id_l_P Γ (π : ev_ctx Γ) : Prop := π `ₑ⊛ a_id = π .
 Lemma sub_id_l_prf : syn_ind_args t_sub_id_l_P v_sub_id_l_P e_sub_id_l_P.
   econstructor.
   all: unfold t_sub_id_l_P, v_sub_id_l_P, e_sub_id_l_P.
   all: intros; cbn; f_equal; auto.
-  all: try rewrite a_shift_id; auto.
+  now rewrite a_shift_id.
 Qed.
 
-Lemma t_sub_id_l {Γ} (t : term Γ) : a_id ⊛ₜ t = t .
+Lemma t_sub_id_l {Γ} (t : term Γ) : t `ₜ⊛ a_id = t .
   now apply (term_ind_mut _ _ _ sub_id_l_prf).
 Qed.
-Lemma v_sub_id_l {Γ} (v : val Γ) : a_id ⊛ᵥ v = v .
+Lemma v_sub_id_l {Γ} (v : val Γ) : v `ᵥ⊛ a_id = v .
   now apply (val_ind_mut _ _ _ sub_id_l_prf).
 Qed.
-Lemma e_sub_id_l {Γ} (π : ev_ctx Γ) : a_id ⊛ₑ π = π .
+Lemma e_sub_id_l {Γ} (π : ev_ctx Γ) : π `ₑ⊛ a_id = π .
   now apply (ctx_ind_mut _ _ _ sub_id_l_prf).
 Qed.
-Lemma m_sub_id_l {Γ} a (v : val_m Γ a) : a_id ⊛ₘ v = v.
+Lemma m_sub_id_l {Γ} a (v : val_m Γ a) : v ᵥ⊛ a_id = v .
   destruct a; [ now apply v_sub_id_l | now apply e_sub_id_l ].
 Qed.
-Lemma s_sub_id_l {Γ} (s : state Γ) : a_id ⊛ₛ s = s.
+Lemma s_sub_id_l {Γ} (s : state Γ) : s ₜ⊛ a_id = s .
   destruct s; cbn; now rewrite t_sub_id_l, e_sub_id_l.
 Qed.
-Lemma a_comp_id_l {Γ1 Γ2} (a : Γ1 =[val_m]> Γ2) : a_id ⊛ a ≡ₐ a .
-  intros ? ?; now apply m_sub_id_l.
-Qed.
 (*|
-Right identity law of substitution.
+Lemma 9: right identity law of substitution. As for renaming, this one is
+mostly by definition.
 |*)
-Lemma m_sub_id_r {Γ1 Γ2} (f : Γ1 =[val_m]> Γ2) {a} (i : Γ1 ∋ a) : f ⊛ₘ a_id a i = f a i.
+Lemma m_sub_id_r {Γ1 Γ2} {a} (i : Γ1 ∋ a) (f : Γ1 =[val_m]> Γ2) : a_id a i ᵥ⊛ f = f a i.
   now destruct a.
 Qed.
-Lemma a_comp_id_r {Γ1 Γ2} (f : Γ1 =[val_m]> Γ2) : f ⊛ a_id ≡ₐ f .
-  intros a ?; now apply m_sub_id_r.
-Qed.
 (*|
-Shifting assigments respects composition.
+Lemma 10: shifting assigments respects composition.
 |*)
-Lemma a_shift_comp {Γ1 Γ2 Γ3 a} (f1 : Γ2 =[val_m]> Γ3) (f2 : Γ1 =[val_m]> Γ2)
-  : @a_shift _ _ a (f1 ⊛ f2) ≡ₐ a_shift f1 ⊛ a_shift f2 .
-  unfold a_shift, m_shift, a_comp, s_map; intros ? h.
-  dependent elimination h; [ symmetry; exact (a_comp_id_r _ _ _) | cbn ].
-  now rewrite m_ren_sub, m_sub_ren.
+Lemma a_shift1_comp {Γ1 Γ2 Γ3 a} (f1 : Γ1 =[val_m]> Γ2) (f2 : Γ2 =[val_m]> Γ3) 
+  : @a_shift1 _ _ a (f1 ⊛ f2) ≡ₐ a_shift1 f1 ⊛ a_shift1 f2 .
+  intros ? v; dependent elimination v; cbn.
+  now rewrite m_sub_id_r.
+  unfold m_shift1; now rewrite m_ren_sub, m_sub_ren.
 Qed.
 (*|
-Substitution-substitution associativity.
+Lemma 11: substitution-substitution associativity, ie composition law.
 |*)
 Definition t_sub_sub_P Γ1 (t : term Γ1) : Prop :=
-  forall Γ2 Γ3 (f1 : Γ2 =[val_m]> Γ3) (f2 : Γ1 =[val_m]> Γ2),
-    f1 ⊛ₜ (f2 ⊛ₜ t) = (f1 ⊛ f2) ⊛ₜ t.
+  forall Γ2 Γ3 (f1 : Γ1 =[val_m]> Γ2) (f2 : Γ2 =[val_m]> Γ3) ,
+  t `ₜ⊛ (f1 ⊛ f2) = (t `ₜ⊛ f1) `ₜ⊛ f2 .
 Definition v_sub_sub_P Γ1 (v : val Γ1) : Prop :=
-  forall Γ2 Γ3 (f1 : Γ2 =[val_m]> Γ3) (f2 : Γ1 =[val_m]> Γ2),
-    f1 ⊛ᵥ (f2 ⊛ᵥ v) = (f1 ⊛ f2) ⊛ᵥ v.
+  forall Γ2 Γ3 (f1 : Γ1 =[val_m]> Γ2) (f2 : Γ2 =[val_m]> Γ3) ,
+  v `ᵥ⊛ (f1 ⊛ f2) = (v `ᵥ⊛ f1) `ᵥ⊛ f2 .
 Definition e_sub_sub_P Γ1 (π : ev_ctx Γ1) : Prop :=
-  forall Γ2 Γ3 (f1 : Γ2 =[val_m]> Γ3) (f2 : Γ1 =[val_m]> Γ2),
-    f1 ⊛ₑ (f2 ⊛ₑ π) = (f1 ⊛ f2) ⊛ₑ π.
+  forall Γ2 Γ3 (f1 : Γ1 =[val_m]> Γ2) (f2 : Γ2 =[val_m]> Γ3) ,
+  π `ₑ⊛ (f1 ⊛ f2) = (π `ₑ⊛ f1) `ₑ⊛ f2 .
 Lemma sub_sub_prf : syn_ind_args t_sub_sub_P v_sub_sub_P e_sub_sub_P.
   econstructor.
   all: unfold t_sub_sub_P, v_sub_sub_P, e_sub_sub_P.
-  all: intros; cbn; f_equal.
-  all: try rewrite a_shift_comp; auto.
+  all: intros; cbn; f_equal; auto.
+  now rewrite a_shift1_comp.
 Qed.
 
-Lemma t_sub_sub {Γ1 Γ2 Γ3} (f1 : Γ2 =[val_m]> Γ3) (f2 : Γ1 =[val_m]> Γ2) (t : term Γ1)
-  : f1 ⊛ₜ (f2 ⊛ₜ t) = (f1 ⊛ f2) ⊛ₜ t.
+Lemma t_sub_sub {Γ1 Γ2 Γ3} (f1 : Γ1 =[val_m]> Γ2) (f2 : Γ2 =[val_m]> Γ3) (t : term Γ1)
+  : t `ₜ⊛ (f1 ⊛ f2) = (t `ₜ⊛ f1) `ₜ⊛ f2 .
   now apply (term_ind_mut _ _ _ sub_sub_prf).
 Qed.
-Lemma v_sub_sub {Γ1 Γ2 Γ3} (f1 : Γ2 =[val_m]> Γ3) (f2 : Γ1 =[val_m]> Γ2) (v : val Γ1)
-  : f1 ⊛ᵥ (f2 ⊛ᵥ v) = (f1 ⊛ f2) ⊛ᵥ v.
+Lemma v_sub_sub {Γ1 Γ2 Γ3} (f1 : Γ1 =[val_m]> Γ2) (f2 : Γ2 =[val_m]> Γ3) (v : val Γ1)
+  : v `ᵥ⊛ (f1 ⊛ f2) = (v `ᵥ⊛ f1) `ᵥ⊛ f2 .
   now apply (val_ind_mut _ _ _ sub_sub_prf).
 Qed.
-Lemma e_sub_sub {Γ1 Γ2 Γ3} (f1 : Γ2 =[val_m]> Γ3) (f2 : Γ1 =[val_m]> Γ2) (π : ev_ctx Γ1)
-  : f1 ⊛ₑ (f2 ⊛ₑ π) = (f1 ⊛ f2) ⊛ₑ π.
+Lemma e_sub_sub {Γ1 Γ2 Γ3} (f1 : Γ1 =[val_m]> Γ2) (f2 : Γ2 =[val_m]> Γ3) (π : ev_ctx Γ1)
+  : π `ₑ⊛ (f1 ⊛ f2) = (π `ₑ⊛ f1) `ₑ⊛ f2 .
   now apply (ctx_ind_mut _ _ _ sub_sub_prf).
 Qed.
-Lemma m_sub_sub {Γ1 Γ2 Γ3} (f1 : Γ2 =[val_m]> Γ3) (f2 : Γ1 =[val_m]> Γ2) a (v : val_m Γ1 a)
-  : f1 ⊛ₘ (f2 ⊛ₘ v) = (f1 ⊛ f2) ⊛ₘ v.
+Lemma m_sub_sub {Γ1 Γ2 Γ3} a (v : val_m Γ1 a) (f1 : Γ1 =[val_m]> Γ2) (f2 : Γ2 =[val_m]> Γ3)
+  : v ᵥ⊛ (f1 ⊛ f2) = (v ᵥ⊛ f1) ᵥ⊛ f2 .
   destruct a; [ now apply v_sub_sub | now apply e_sub_sub ].
 Qed.
-Lemma s_sub_sub {Γ1 Γ2 Γ3} (f1 : Γ2 =[val_m]> Γ3) (f2 : Γ1 =[val_m]> Γ2) (s : state Γ1)
-  : f1 ⊛ₛ (f2 ⊛ₛ s) = (f1 ⊛ f2) ⊛ₛ s.
+Lemma s_sub_sub {Γ1 Γ2 Γ3} (s : state Γ1) (f1 : Γ1 =[val_m]> Γ2) (f2 : Γ2 =[val_m]> Γ3) 
+  : s ₜ⊛ (f1 ⊛ f2) = (s ₜ⊛ f1) ₜ⊛ f2 .
   destruct s; cbn; now rewrite t_sub_sub, e_sub_sub.
 Qed.
-Lemma a_comp_assoc {Γ1 Γ2 Γ3 Γ4} (u : Γ3 =[val_m]> Γ4) (v : Γ2 =[val_m]> Γ3) (w : Γ1 =[val_m]> Γ2)
-           : u ⊛ (v ⊛ w) ≡ₐ (u ⊛ v) ⊛ w .
-  intros ? ?; unfold a_comp; now apply m_sub_sub.
-Qed.
 Lemma a_sub1_sub {Γ Δ a} (f : Γ =[val_m]> Δ) (v : val_m Γ a)
-  : assign1 (f ⊛ₘ v) ⊛ a_shift f ≡ₐ f ⊛ (assign1 v).
-
-  intros ? h; unfold a_comp, s_map.
-  dependent elimination h; [ cbn; now rewrite m_sub_id_r | ].
-  cbn; unfold s_map, m_shift; rewrite m_sub_ren, m_sub_id_r.
-  now apply m_sub_id_l.
+  : a_shift1 f ⊛ assign1 (v ᵥ⊛ f) ≡ₐ (assign1 v) ⊛ f .
+  intros ? i; dependent elimination i; cbn.
+  now rewrite m_sub_id_r.
+  unfold m_shift1; rewrite m_sub_ren, m_sub_id_r; now apply m_sub_id_l.
 Qed.
-Lemma t_sub1_sub {Γ Δ x} (f : Γ =[val_m]> Δ) (t : term (Γ ▶ x)) v
-  : t_subst (a_shift f) t /[ m_subst f _ v ] = t_subst f (t /[ v ]) .
-  unfold t_subst1; now rewrite 2 t_sub_sub, a_sub1_sub.
+Lemma t_sub1_sub {Γ Δ x} (f : Γ =[val_m]> Δ) (t : term (Γ ▶ₓ x)) v
+  : (t `ₜ⊛ a_shift1 f) /[ v ᵥ⊛ f ] = (t /[ v ]) `ₜ⊛ f.
+  unfold t_subst1; now rewrite <- 2 t_sub_sub, a_sub1_sub.
 Qed.
 (*|
 The Actual Instance
 -------------------
 
-We can now instanciate our framework with untyped lambda calculus.
+We can now instanciate the generic OGS construction.
 |*)
-#[local] Instance ulc_typ  : baseT := {| typ := ty |}.
-
-#[local] Instance ulc_spec : observation_structure :=
-  {| Obs.obs := obs ;
-     dom := @obs_dom |} .
-
-#[local] Instance ulc_val  : baseV :=
-  {| Subst.val := val_m |}.
-#[local] Instance ulc_val_mon : subst_monoid _ :=
-  {| v_var := @a_id ;
-     v_sub := @m_subst |} .
-#[local] Instance ulc_val_laws : subst_monoid_laws :=
+#[global] Instance ulc_val_laws : subst_monoid_laws val_m :=
   {| v_sub_proper := @m_sub_eq ;
-     v_sub_var := @a_comp_id_r ;
-     v_var_sub := @a_comp_id_l ;
-     Subst.v_sub_sub := @a_comp_assoc |} .
+     v_sub_var := @m_sub_id_r ;
+     v_var_sub := @m_sub_id_l ;
+     Subst.v_sub_sub := @m_sub_sub |} .
 
-#[local] Instance ulc_conf : baseC :=
-  {| Subst.conf := state |}.
-#[local] Instance ulc_conf_mod : subst_module _ _ :=
-  {| c_sub := @s_subst |} .
-#[local] Instance ulc_conf_laws : subst_module_laws :=
+#[global] Instance ulc_conf_laws : subst_module_laws val_m state :=
   {| c_sub_proper := @s_sub_eq ;
      c_var_sub := @s_sub_id_l ;
      c_sub_sub := @s_sub_sub |} .
 
-#[local] Instance ulc_var_laws : var_assumptions.
-  econstructor; intros.
-  - destruct x; now dependent induction H.
-  - destruct x; induction v; try (apply inr; intros [ i H ]; now inversion H).
-    all: apply inl; econstructor; auto.
-  - destruct X as [ i H ].
-    destruct x; induction v; try now inversion H.
-    all: refine (h ,' eq_refl).
-Defined.
+#[global] Instance ulc_var_laws : var_assumptions val_m.
+  econstructor.
+  - intros ? [] ?? H; now dependent destruction H.
+  - intros ? [] []; try now apply Yes; exact (Vvar _).
+    all: apply No; intro H; dependent destruction H.
+  - intros ?? [] v r H; induction v; dependent destruction H; exact (Vvar _).
+Qed.
 
-#[local] Instance ulc_machine : machine :=
+#[global] Instance ulc_machine : machine val_m state obs_op :=
   {| eval := @ulc_eval ;
-     app := @obs_app |} .
+     oapp := @obs_app |} .
 
-(*|
-We now prove the remaining hypotheses of the machine.
-We pull in some tooling for coinductive reasoning on the delay monad.
-|*)
 From Coinduction Require Import coinduction lattice rel tactics.
 From OGS.ITree Require Import Eq.
 
-#[local] Instance ulc_machine_law : machine_laws.
-  econstructor; intros; unfold ulc_spec, ulc_val in *; cbn in *.
-(*|
-Applying an observation respects pointwise equality of assigments.
-|*)
-  - intros ? ? H1; dependent elimination m; cbn; repeat (f_equal; auto).
-(*|
-Applying an observation commutes with renamings.
-|*)
-  - destruct x; dependent elimination m; cbn; f_equal.
-(*|
-Evaluation respects substitution.
-|*)
-  - revert c e; unfold comp_eq, it_eq; coinduction R CIH; intros c e.
-    destruct c. cbn in e0.
-    dependent elimination t.
-    * dependent elimination e0.
-      + unfold ulc_eval at 2; cbn - [ ulc_eval ];
-          change (it_eqF _ ?a ?b T1_0 (observe ?x) (_observe ?y)) with (it_eq_bt _ a R T1_0 x y).
-        refine (gfp_bt (it_eq_map _ _) R T1_0 _ _ _); reflexivity.
-      + cbn; econstructor;
-          change (Structure.iter _ _ ?a) with (ulc_eval a);
-          change (Structure.subst (fun pat : T1 => let 'T1_0 := pat in ?f) T1_0 ?u) with (bind_delay' u f).
-        exact (CIH (Cut t0 (K2 v e0)) e).
-      + dependent elimination v.
-        ++ unfold ulc_eval at 2; cbn - [ ulc_eval ];
-             change (it_eqF _ ?a _ T1_0 (observe ?x) (_observe ?y)) with (it_eq_bt _ a R T1_0 x y).
-           refine (gfp_bt (it_eq_map _ _) R T1_0 _ _ _); reflexivity.
-        ++ cbn; econstructor;
-           change (v_subst e ?a) with (m_subst e (⊕) a); rewrite t_sub1_sub.
-           exact (CIH (Cut (t0 /[ v0 ]) e1) e).
-    * cbn; econstructor.
-      exact (CIH (Cut t1 (K1 t0 e0)) e).
-(*|
-Evaluating a normal form yields the same normal form instantly.
-|*)
-  - destruct u as [ a [ i [ p γ ] ]].
-    unfold nf'_ty, nf'_var, nf'_val, a_id; cbn in *.
-    destruct a; dependent elimination p; cbn in *.
+Ltac refold_eval :=
+  change (Structure.iter _ _ ?a) with (ulc_eval a);
+  change (Structure.subst (fun pat : T1 => let 'T1_0 := pat in ?f) T1_0 ?u)
+    with (bind_delay' u f).
+
+#[global] Instance ulc_machine_law : machine_laws val_m state obs_op.
+  econstructor; cbn; intros.
+  - intros ?? H1; dependent elimination o; cbn; repeat (f_equal; auto).
+  - destruct x; dependent elimination o; cbn; f_equal.
+  - revert c a; unfold comp_eq, it_eq; coinduction R CIH; intros c e.
+    cbn; funelim (eval_step c); cbn.
+    + destruct (e (⊖) i); auto.
+      remember (v `ᵥ⊛ e) as v'; clear H v Heqv'.
+      dependent elimination v'; cbn; auto.
+    + econstructor; refold_eval; apply CIH.
+    + remember (e (⊕) i) as vv; clear H i Heqvv.
+      dependent elimination vv; cbn; auto.
+    + econstructor;
+       refold_eval;
+       change (?v `ᵥ⊛ ?a) with ((v : val_m _ (⊕)) ᵥ⊛ a).
+      rewrite t_sub1_sub.
+      apply CIH.
+    + econstructor; refold_eval; apply CIH.
+  - destruct u as [ a i [ p γ ] ]; cbn.
+    dependent elimination p; cbn.
     all: unfold comp_eq; apply it_eq_unstep; cbn; econstructor.
-    all: do 3 (unshelve econstructor; auto; cbn).
-    all: intros ? h; do 3 (dependent elimination h; auto).
-(*|
-The language "has finite redexes" (wellfoundedness of the head instanciation relation).
-|*)
+    all: econstructor; intros ? v; do 3 (dependent elimination v; auto).
   - intros [ x p ].
     destruct x; dependent elimination p; econstructor.
     * intros [ z p ] H.
-      destruct z; dependent elimination p; dependent elimination H.
-      + dependent elimination v; try now destruct (p (_ ,' eq_refl)).
-        apply it_eq_step in i0; now inversion i0.
-      + dependent elimination v; try now destruct (p (_ ,' eq_refl)).
-        apply it_eq_step in i0; now inversion i0.
+      dependent elimination p; dependent elimination H.
+      all: dependent elimination v; try now destruct (t0 (Vvar _)).
+      all: apply it_eq_step in i0; now inversion i0.
     * intros [ z p ] H.
-      destruct z; dependent elimination p; dependent elimination H.
-      + cbn in *.
-        pose (vv :=e (⊕) Ctx.top); change (e (⊕) Ctx.top) with vv in i0; remember vv; clear vv Heqv0 e.
-        dependent elimination v; try now destruct (p (_ ,' eq_refl)).
-        apply it_eq_step in i0; now inversion i0.
-        dependent elimination v0; apply it_eq_step in i0; cbn in i0; dependent elimination i0.
-        unfold obs'_of_nf' in r_rel; cbn in r_rel.
-        inversion_sigma r_rel; dependent elimination r_rel1; clear .
-        econstructor; intros [ z p ] H.
-        destruct z; dependent elimination p; dependent elimination H.
-        ++ dependent elimination v; try now destruct (p (_ ,' eq_refl)).
-           apply it_eq_step in i0; now inversion i0.
-        ++ dependent elimination v; try now destruct (p (_ ,' eq_refl)).
-           apply it_eq_step in i0; now inversion i0.
-      + cbn in *.
-        pose (vv :=e (⊕) Ctx.top); change (e (⊕) Ctx.top) with vv in i0; remember vv; clear vv Heqv0 e.
-        dependent elimination v; try now destruct (p (_ ,' eq_refl)).
-        apply it_eq_step in i0; now inversion i0.
-        dependent elimination v0; apply it_eq_step in i0; cbn in i0; dependent elimination i0.
-        unfold obs'_of_nf' in r_rel; cbn in r_rel.
-        inversion_sigma r_rel; inversion r_rel1.
+      dependent elimination p; dependent elimination H; cbn in *.
+      dependent elimination v; try now destruct (t0 (Vvar _)).
+      + apply it_eq_step in i0; now inversion i0.
+      + remember (a _ Ctx.top) as vv; clear a Heqvv.
+        dependent elimination vv;
+          apply it_eq_step in i0; cbn in i0; dependent elimination i0.
+        inversion r_rel.
+      + econstructor; intros [ z p ] H.
+        dependent elimination p; dependent elimination H.
+        all: dependent elimination v0; try now destruct (t1 (Vvar _)).
+        all: apply it_eq_step in i2; now inversion i2.
 Qed.
 (*|
-And this is it. Lets instanciate the notions to enjoy a nice readable type for our theorem.
+Concrete soundness theorem
+--------------------------
 |*)
 Definition subst_eq Δ {Γ} : relation (state Γ) :=
-  fun u v => forall σ : Γ =[val_m]> Δ, eval_to_obs (σ ⊛ₛ u) ≈ eval_to_obs (σ ⊛ₛ v) .
-Notation "x ≈[sub Δ ]≈ y" := (subst_eq Δ x y) (at level 10).
-(*|
-Our semantic objects live in what is defined in the generic construction as
-`ogs_act`, that is active strategies for the OGS game. They come with their
-own notion of equivalence, weak bisimilarity and we get to interpret states
-into semantic objects.
-|*)
-Definition sem_act Δ Γ := ogs_act Δ (∅ ▶ Γ) .
+  fun u v => forall σ : Γ =[val_m]> Δ, evalₒ (u ₜ⊛ σ) ≈ evalₒ (v ₜ⊛ σ) .
+Notation "x ≈⟦sub Δ ⟧≈ y" := (subst_eq Δ x y) (at level 10).
 
-Definition ogs_weq_act Δ {Γ} : relation (sem_act Δ Γ) := fun u v => u ≈ v .
-Notation "u ≈[ogs Δ ]≈ v" := (ogs_weq_act Δ u v) (at level 40).
-
-Definition interp_act_s Δ {Γ} (c : state Γ) : sem_act Δ Γ := m_strat (∅ ▶ Γ) (inj_init_act Δ c) .
-Notation "⟦ t ⟧ₛ" := (interp_act_s _ t) .
-(*|
-We can now obtain our instance of the correctness result!
-|*)
 Theorem ulc_subst_correct Δ {Γ} (x y : state Γ)
-  : ⟦ x ⟧ₛ ≈[ogs Δ ]≈ ⟦ y ⟧ₛ -> x ≈[sub Δ ]≈ y .
+  : x ≈⟦ogs Δ⟧≈ y -> x ≈⟦sub Δ⟧≈ y .
   exact (ogs_correction Δ x y).
 Qed.
 (*|
@@ -835,44 +725,86 @@ Recovering CIU-equivalence
 |*)
 Definition ciu_eq Δ {Γ} : relation (term Γ) :=
   fun u v => forall (σ : Γ =[val_m]> Δ) (π : ev_ctx Δ),
-      eval_to_obs (Cut (σ ⊛ₜ u) π) ≈ eval_to_obs (Cut (σ ⊛ₜ v) π) .
-Notation "x ≈[ciu Δ ]≈ y" := (ciu_eq Δ x y) (at level 10).
-(*|
-Embedding terms into states.
-|*)
-Definition c_init {Γ} (t : term Γ) : state (Γ ▶ ⊖)
-  := Cut (t_shift t) (K0 Ctx.top) .
-Notation "⟦ t ⟧ₜ" := (⟦ c_init t ⟧ₛ) .
-(*|
-Embedding evaluation context and assignment into generalized assignments.
-|*)
+      evalₒ (Cut (u `ₜ⊛ σ) π) ≈ evalₒ (Cut (v `ₜ⊛ σ) π) .
+Notation "x ≈⟦ciu Δ ⟧≈ y" := (ciu_eq Δ x y) (at level 10).
+
+Definition c_init {Γ} (t : term Γ) : state (Γ ▶ₓ ⊖)
+  := Cut (t_shift1 t) (K0 Ctx.top) .
+
 Definition a_of_sk {Γ Δ} (σ : Γ =[val_m]> Δ) (π : ev_ctx Δ)
-  : (Γ ▶ ⊖) =[val_m]> Δ := σ ▶ₐ (π : val_m _ (⊖)) .
-(*|
-Relating the two previous embeddings with substitution.
-|*)
+  : (Γ ▶ₓ ⊖) =[val_m]> Δ := σ ▶ₐ (π : val_m _ (⊖)) .
+
 Lemma sub_init {Γ Δ} (t : term Γ) (σ : Γ =[val_m]> Δ) (π : ev_ctx Δ)
-  : Cut (σ ⊛ₜ t) π = a_of_sk σ π ⊛ₛ c_init t .
-  cbn; unfold t_shift; now rewrite t_sub_ren.
+  : Cut (t `ₜ⊛ σ) π = c_init t ₜ⊛ a_of_sk σ π  .
+  cbn; unfold t_shift1; now rewrite t_sub_ren.
 Qed.
 (*|
-The more standard CIU statement for terms.
+We can now obtain a correctness theorem with respect to standard
+CIU-equivalence by embedding terms into states. Proving that CIU-equivalence
+entails our substitution equivalence is left to the reader!
 |*)
-Theorem ulc_ciu_correct Δ {Γ} (x y : term Γ)
-  : ⟦ x ⟧ₜ ≈[ogs Δ ]≈ ⟦ y ⟧ₜ -> x ≈[ciu Δ ]≈ y .
+Theorem stlc_ciu_correct Δ {Γ} (x y : term Γ)
+  : c_init x ≈⟦ogs Δ⟧≈ c_init y -> x ≈⟦ciu Δ⟧≈ y .
   intros H σ k; rewrite 2 sub_init.
   now apply ulc_subst_correct.
 Qed.
+
 (*|
-Some bonus example terms.
+Example terms
+-------------
+
+Following a trick by Conor McBride we provide a cool notation for writing terms
+without any DeBruijn indices, instead leveraging Coq's binders. For this we need
+a bit of infrastructure, for manipulating terms that only have term variables.
 |*)
-Module ExampleTerms.
+Equations n_ctx : nat -> t_ctx :=
+  n_ctx O     := ∅ ;
+  n_ctx (S n) := n_ctx n ▶ₓ ⊕ .
+
+Notation var' n := (n_ctx n ∋ ⊕).
+Notation term' n := (term (n_ctx n)).
+
+Equations v_emb (n : nat) : var' (S n) :=
+  v_emb O     := Ctx.top ;
+  v_emb (S n) := pop (v_emb n) .
+
+Equations v_lift {n} : var' n -> var' (S n) :=
+  @v_lift (S _) Ctx.top     := Ctx.top ;
+  @v_lift (S _) (pop i) := pop (v_lift i) .
 (*|
-λx.xx
+Here starts the magic.
 |*)
-Definition t_self_app : term ∅ := Val (Lam (App (Val (Var Ctx.top)) (Val (Var Ctx.top)))) .
+Equations mk_var (m : nat) : forall n, var' (m + S n) :=
+  mk_var O     := v_emb ;
+  mk_var (S m) := v_lift ∘ mk_var m .
+
+Definition mk_lam {m : nat} (f : (forall n, term' (m + S n)) -> term' (S m)) : term' m
+  := Val (Lam (f (Val ∘ Var ∘ mk_var m))).
+Arguments mk_lam {_} & _ .
 (*|
-`Ω = (λx.xx)(λx.xx)
+Now a bit of syntactic sugar.
 |*)
-Definition t_omega : term ∅ := App t_self_app t_self_app .
-End ExampleTerms.
+Declare Custom Entry lambda.
+Notation "✨ e ✨" := (e : term' 0) (e custom lambda at level 2).
+Notation "x" := (x _) (in custom lambda at level 0, x ident).
+Notation "( x )" := x (in custom lambda at level 0, x at level 2).
+Notation "x y" := (App x y)
+  (in custom lambda at level 1, left associativity).
+Notation "'λ' x .. y ⇒ U" :=
+  (mk_lam (fun x => .. (mk_lam (fun y => U)) ..))
+  (in custom lambda at level 1, x binder, y binder, U at level 2).
+(*|
+Aren't these beautiful?
+|*)
+Definition Delta := ✨ (λ x ⇒ x x) ✨ .
+Definition Omega := ✨ (λ x ⇒ x x) (λ x ⇒ x x) ✨ .
+Definition Upsilon := ✨ λ f ⇒ (λ x ⇒ f (x x)) (λ x ⇒ f (x x)) ✨.
+Definition Theta := ✨ (λ x f ⇒ f (x x f)) (λ x f ⇒ f (x x f)) ✨.
+(*|
+You can check the actual lambda-term they unwrap to
+by running eg:
+
+.. coq::
+
+  Eval cbv in Upsilon.
+|*)
